Busybeaver/Reachability.lean
@@ -624,3 +624,98 @@ def Machine.stepH
   }⟩
 
 end TM
+
+namespace TM.Model
+
+variable {M : Type _} [TM.Model M]
+
+inductive Multistep (m : M) : Nat → Config M → Config M → Prop
+| refl {C} : Multistep m 0 C C
+| step {i j A B C} :
+    StepRel m i A B →
+    Multistep m j B C →
+    Multistep m (i + j) A C
+
+inductive HaltRel (m : M) : Nat → Config M → Config M → Prop
+| halt {k A B} : SegmentHaltRel m k A B → HaltRel m k A B
+| step {i j A B C} :
+    StepRel m i A B →
+    HaltRel m j B C →
+    HaltRel m (i + j) A C
+
+def halts_in (m : M) (k : Nat) (A : Config M) : Prop := ∃ C, HaltRel m k A C
+
+def halts (m : M) (A : Config M) : Prop := ∃ k, halts_in m k A
+
+namespace Multistep
+
+lemma single {m : M} (hAB : StepRel m k A B) : Multistep m k A B := by
+  exact .step hAB .refl
+
+lemma trans {m : M} (hAB : Multistep m i A B) (hBC : Multistep m j B C) :
+    Multistep m (i + j) A C := by
+  induction hAB with
+  | refl =>
+      simpa using hBC
+  | @step i j A B D hAB hBD IH =>
+      simpa [Nat.add_assoc] using
+        Multistep.step hAB (IH hBC)
+
+end Multistep
+
+namespace HaltRel
+
+lemma to_halts_in {m : M} (h : HaltRel m k A B) : halts_in m k A := ⟨B, h⟩
+
+lemma to_halts {m : M} (h : HaltRel m k A B) : halts m A := ⟨k, h.to_halts_in⟩
+
+lemma trans_multistep {m : M} (hAB : Multistep m i A B) (hBC : HaltRel m j B C) :
+    HaltRel m (i + j) A C := by
+  induction hAB with
+  | refl =>
+      simpa using hBC
+  | @step i j A B D hAB hBD IH =>
+      simpa [Nat.add_assoc] using
+        HaltRel.step hAB (IH hBC)
+
+lemma of_lastConfig {m : M} (h : LastConfig m A) : HaltRel m 0 A A := by
+  apply HaltRel.halt
+  have hzero : (TM.Model.step m A).baseSteps = 0 := (TM.Model.step_zero_iff m A).mpr h
+  cases hstep : TM.Model.step m A with
+  | mk baseSteps outcome =>
+      simp [LastConfig] at h
+      simp [hstep] at hzero h
+      cases outcome
+      · cases h
+      · cases h
+        simp [SegmentHaltRel, hstep, hzero]
+
+end HaltRel
+
+inductive HaltM (m : M) (α : Type _)
+| unknown : α → HaltM m α
+| halts_prf : ∀ k C, HaltRel m k (init M) C → HaltM m α
+| loops_prf : ¬halts m (init M) → HaltM m α
+
+namespace HaltM
+
+variable {m : M} {α : Type _}
+
+instance (m : M) : Monad (HaltM m) where
+  pure := .unknown
+  bind := fun x f =>
+    match x with
+    | .unknown v => f v
+    | .halts_prf k C h => .halts_prf k C h
+    | .loops_prf h => .loops_prf h
+
+def decided : HaltM m α → Bool
+| .unknown _ => false
+| _ => true
+
+end HaltM
+
+abbrev GDecider (M : Type _) [TM.Model M] :=
+  (m : M) → HaltM m Unit
+
+end TM.Model
